ConcreteToSymbolicLemmas.v
@@ -16,7 +16,7 @@ From MyProject Require Import CrProgramState.
 
 (* Simpler lemma with no state update *)
 Lemma commute_sym_conc_expr:
-  forall (ho: HdrOp) (s : ProgramState SmtArithExpr) (f : SmtValuation),
+  forall (ho: HdrOp) (s : SymbolicState) (f : SmtValuation),
     eval_hdr_op_expr_uint8 ho (eval_sym_state s f) =
     eval_smt_arith (eval_hdr_op_expr_smt ho s) f.
 Proof.
@@ -28,7 +28,7 @@ Proof.
 Qed.
 
 Lemma commute_update_eval_state:
-  forall (s : ProgramState SmtArithExpr) (f : SmtValuation) (sv : StateVar) (v : SmtArithExpr),
+  forall (s : SymbolicState) (f : SmtValuation) (sv : StateVar) (v : SmtArithExpr),
     eval_sym_state (update_state s sv v) f =
     update_state (eval_sym_state s f) sv (eval_smt_arith v f).
 Proof.
@@ -40,7 +40,7 @@ Proof.
 Qed.
 
 Lemma commute_update_eval_hdr:
-  forall (s : ProgramState SmtArithExpr) (f : SmtValuation) (h : Header) (v : SmtArithExpr),
+  forall (s : SymbolicState) (f : SmtValuation) (h : Header) (v : SmtArithExpr),
     eval_sym_state (update_hdr s h v) f =
     update_hdr (eval_sym_state s f) h (eval_smt_arith v f).
 Proof.
@@ -55,7 +55,7 @@ Qed.
   concretizing and then evaluating EQUALS
   evaluating and then concretizing *)
 Lemma commute_sym_conc_assign:
-  forall (ho : HdrOp) (s : ProgramState SmtArithExpr) (f : SmtValuation),
+  forall (ho : HdrOp) (s : SymbolicState) (f : SmtValuation),
      eval_hdr_op_assign_uint8 ho (eval_sym_state s f) =
       eval_sym_state (eval_hdr_op_assign_smt ho s) f.
 Proof.
@@ -69,8 +69,8 @@ Qed.
 
 Lemma commute_sym_vs_conc_hdr_op_list :
   forall (hol : list HdrOp) (f : SmtValuation)
-         (s1 : ProgramState SmtArithExpr)
-         (c1 : ProgramState uint8),
+         (s1 : SymbolicState)
+         (c1 : ConcreteState),
     c1 = eval_sym_state s1 f ->
     eval_hdr_op_list_uint8 hol c1 = (* first concretize, and then interpret *) 
     eval_sym_state (eval_hdr_op_list_smt hol s1) f.    (* first interpret, and then concretize *)
@@ -87,8 +87,8 @@ Qed.
    concrete and symbolic execution match up. *)
 Lemma commute_sym_vs_conc_match_cond :
   forall (hv_pair: Header * uint8) (f : SmtValuation)
-         (s1 : ProgramState SmtArithExpr)
-         (c1 : ProgramState uint8),
+         (s1 : SymbolicState)
+         (c1 : ConcreteState),
     c1 = eval_sym_state s1 f ->
     eval_match_uint8 [hv_pair] c1 = (* first concretize, and then interpret *)
     eval_smt_bool (eval_match_smt [hv_pair] s1) f. (* first interpret, and then concretize *)
@@ -114,8 +114,8 @@ Qed.
    generalized to a MatchPattern instead of a header_pair *)
 Lemma commute_sym_vs_conc_match_pattern :
   forall (mp: MatchPattern) (f : SmtValuation)
-         (s1 : ProgramState SmtArithExpr)
-         (c1 : ProgramState uint8),
+         (s1 : SymbolicState)
+         (c1 : ConcreteState),
     c1 = eval_sym_state s1 f ->
     eval_match_uint8 mp c1 = (* first concretize, and then interpret *)
     eval_smt_bool (eval_match_smt mp s1) f. (* first interpret , and then concretize *)
@@ -143,7 +143,7 @@ Qed.
 
 Lemma commute_sym_vs_conc_helper_seq_par_rule_hdr :
   forall (mp: MatchPattern) (hol: list HdrOp) (f : SmtValuation)
-         (s1 : ProgramState SmtArithExpr) (h : Header),
+         (s1 : SymbolicState) (h : Header),
          is_header_in_ps s1 h <> None ->
     lookup_hdr (if eval_match_uint8 mp (eval_sym_state s1 f)
     then eval_hdr_op_list_uint8 hol (eval_sym_state s1 f)
@@ -176,7 +176,7 @@ Qed.
 
 Lemma commute_sym_vs_conc_helper_seq_par_rule_sv :
   forall (mp: MatchPattern) (hol: list HdrOp) (f : SmtValuation)
-         (s1 : ProgramState SmtArithExpr) (sv : StateVar),
+         (s1 : SymbolicState) (sv : StateVar),
          is_state_var_in_ps s1 sv <> None ->
     lookup_state (if eval_match_uint8 mp (eval_sym_state s1 f)
     then eval_hdr_op_list_uint8 hol (eval_sym_state s1 f)
@@ -208,7 +208,7 @@ Qed.
 
 Lemma commute_sym_vs_conc_seq_rule_hdr :
   forall (sr: SeqRule) (f : SmtValuation)
-         (s1 : ProgramState SmtArithExpr) (h : Header),
+         (s1 : SymbolicState) (h : Header),
       is_header_in_ps s1 h <> None ->
       lookup_hdr (eval_seq_rule_uint8 sr (eval_sym_state s1 f)) h = (* first concretize, and then interpret *)
       lookup_hdr (eval_sym_state (eval_seq_rule_smt sr s1) f) h. (* first interpret, and then concretize *)
@@ -222,7 +222,7 @@ Qed.
 
 Lemma commute_sym_vs_conc_par_rule_hdr :
   forall (pr: ParRule) (f : SmtValuation)
-         (s1 : ProgramState SmtArithExpr) (h : Header),
+         (s1 : SymbolicState) (h : Header),
     is_header_in_ps s1 h <> None ->
     lookup_hdr (eval_par_rule_uint8 pr (eval_sym_state s1 f)) h = (* first concretize, and then interpret *)
     lookup_hdr (eval_sym_state (eval_par_rule_smt pr s1) f) h. (* first interpret, and then concretize *)
@@ -237,7 +237,7 @@ Qed.
 (* Same as above two lemmas but for state variables *)
 Lemma commute_sym_vs_conc_seq_rule_sv :
   forall (sr: SeqRule) (f : SmtValuation)
-         (s1 : ProgramState SmtArithExpr) (sv : StateVar),
+         (s1 : SymbolicState) (sv : StateVar),
     is_state_var_in_ps s1 sv <> None ->
     lookup_state (eval_seq_rule_uint8 sr (eval_sym_state s1 f)) sv = (* first concretize, and then interpret *)
     lookup_state (eval_sym_state (eval_seq_rule_smt sr s1) f) sv. (* first interpret, and then concretize *)
@@ -251,7 +251,7 @@ Qed.
 
 Lemma commute_sym_vs_conc_par_rule_sv :
   forall (pr: ParRule) (f : SmtValuation)
-         (s1 : ProgramState SmtArithExpr) (sv : StateVar),
+         (s1 : SymbolicState) (sv : StateVar),
     is_state_var_in_ps s1 sv <> None ->
     lookup_state (eval_par_rule_uint8 pr (eval_sym_state s1 f)) sv = (* first concretize, and then interpret *)
     lookup_state (eval_sym_state (eval_par_rule_smt pr s1) f) sv. (* first interpret, and then concretize *)
@@ -265,7 +265,7 @@ Qed.
 
 Lemma commute_sym_vs_conc_ma_rule_hdr:
   forall (ma : MatchActionRule) (f : SmtValuation)
-         (s1 : ProgramState SmtArithExpr) (h: Header),
+         (s1 : SymbolicState) (h: Header),
     is_header_in_ps s1 h <> None ->
     lookup_hdr (eval_match_action_rule_uint8 ma (eval_sym_state s1 f)) h = (* first concretize, and then interpret *)
     lookup_hdr (eval_sym_state (eval_match_action_rule_smt ma s1) f) h. (* first interpret, and then concretize *)
@@ -278,7 +278,7 @@ Qed.
 
 Lemma commute_sym_vs_conc_ma_rule_sv:
   forall (ma : MatchActionRule) (f : SmtValuation)
-         (s1 : ProgramState SmtArithExpr) (sv: StateVar),
+         (s1 : SymbolicState) (sv: StateVar),
     is_state_var_in_ps s1 sv <> None ->
     lookup_state (eval_match_action_rule_uint8 ma (eval_sym_state s1 f)) sv = (* first concretize, and then interpret *)
     lookup_state (eval_sym_state (eval_match_action_rule_smt ma s1) f) sv. (* first interpret, and then concretize *)
@@ -324,7 +324,7 @@ Lemma switch_case_expr_some_match_lemma :
     Some rule = find_first_match (combine (get_match_results t (eval_sym_state s1 f)) t) ->
     lookup_hdr (eval_match_action_rule_uint8 rule (eval_sym_state s1 f)) h =
     eval_smt_arith (switch_case_expr (combine (get_match_results_smt t s1)
-                                              (map (fun ps : ProgramState SmtArithExpr => lookup_hdr ps h)
+                                              (map (fun ps : SymbolicState => lookup_hdr ps h)
                                                    (map (fun rule : MatchActionRule => eval_match_action_rule_smt rule s1) t)))
                                      (lookup_hdr s1 h)) f.
 Proof.
@@ -385,7 +385,7 @@ Lemma switch_case_expr_no_match_lemma :
     None = find_first_match (combine (get_match_results t (eval_sym_state s1 f)) t) ->
     eval_smt_arith (lookup_hdr s1 h) f =
     eval_smt_arith (switch_case_expr  (combine (get_match_results_smt t s1)
-                                               (map (fun ps : ProgramState SmtArithExpr => lookup_hdr ps h)
+                                               (map (fun ps : SymbolicState => lookup_hdr ps h)
                                                     (map (fun rule : MatchActionRule => eval_match_action_rule_smt rule s1) t)))
                                       (lookup_hdr s1 h)) f.
 Proof.
@@ -441,7 +441,7 @@ Lemma switch_case_expr_some_match_state_var_lemma :
     Some rule = find_first_match (combine (get_match_results t (eval_sym_state s1 f)) t) ->
     lookup_state (eval_match_action_rule_uint8 rule (eval_sym_state s1 f)) sv =
     eval_smt_arith (switch_case_expr (combine (get_match_results_smt t s1)
-                                              (map (fun ps : ProgramState SmtArithExpr => lookup_state ps sv)
+                                              (map (fun ps : SymbolicState => lookup_state ps sv)
                                                    (map (fun rule : MatchActionRule => eval_match_action_rule_smt rule s1) t)))
                                      (lookup_state s1 sv)) f.
 Proof.
@@ -504,7 +504,7 @@ Lemma switch_case_expr_no_match_state_var_lemma :
     None = find_first_match (combine (get_match_results t (eval_sym_state s1 f)) t) ->
     eval_smt_arith (lookup_state s1 sv) f =
     eval_smt_arith (switch_case_expr  (combine (get_match_results_smt t s1)
-                                               (map (fun ps : ProgramState SmtArithExpr => lookup_state ps sv)
+                                               (map (fun ps : SymbolicState => lookup_state ps sv)
                                                     (map (fun rule : MatchActionRule => eval_match_action_rule_smt rule s1) t)))
                                       (lookup_state s1 sv)) f.
 Proof.
@@ -557,7 +557,7 @@ Lemma hdr_transformer_helper:
      (lookup_hdr (eval_transformer_smt t s1) h) =
      switch_case_expr
      (combine (get_match_results_smt t s1)
-     (map (fun ps : ProgramState SmtArithExpr => lookup_hdr ps h)
+     (map (fun ps : SymbolicState => lookup_hdr ps h)
      (map (fun rule : MatchActionRule => eval_match_action_rule_smt rule s1) t)))
      (lookup_hdr s1 h).
 Proof.
@@ -599,7 +599,7 @@ Lemma state_transformer_helper:
      (lookup_state (eval_transformer_smt t s1) sv) =
      switch_case_expr
      (combine (get_match_results_smt t s1)
-     (map (fun ps : ProgramState SmtArithExpr => lookup_state ps sv)
+     (map (fun ps : SymbolicState => lookup_state ps sv)
      (map (fun rule : MatchActionRule => eval_match_action_rule_smt rule s1) t)))
      (lookup_state s1 sv).
 Proof.
@@ -648,7 +648,7 @@ Qed.
 
 Lemma commute_sym_vs_conc_transfomer_hdr:
   forall (t: Transformer) (f : SmtValuation)
-         (s1 : ProgramState SmtArithExpr)
+         (s1 : SymbolicState)
          (h : Header),
     is_header_in_ps s1 h <> None ->
     lookup_hdr (eval_transformer_uint8 t (eval_sym_state s1 f)) h = (* first concretize, and then interpret *)
@@ -669,7 +669,7 @@ Qed.
 
 Lemma commute_sym_vs_conc_transfomer_sv:
   forall (t: Transformer) (f : SmtValuation)
-         (s1 : ProgramState SmtArithExpr)
+         (s1 : SymbolicState)
          (sv : StateVar),
     is_state_var_in_ps s1 sv <> None ->
     lookup_state (eval_transformer_uint8 t (eval_sym_state s1 f)) sv = (* first concretize, and then interpret *)
