SmtExpr.v
@@ -1,7 +1,6 @@
 (* Write out semantics for bitvectors in SMT,
    show that a single hdr_op evaluation can be converted to the appropriate SMT formula in Z3 *)
 From MyProject Require Import CrIdentifiers.
-From MyProject Require Import CrProgramState.
 From Coq.Strings Require Import String.
 
 (* Note that these strings may or may not have a one-to-one correspondence with
@@ -62,8 +61,3 @@ with eval_smt_arith (e : SmtArithExpr) (v : SmtValuation) : uint8 :=
     | SmtBitDiv e1 e2 => divu (eval_smt_arith e1 v) (eval_smt_arith e2 v)
     | SmtBitMod e1 e2 => modu (eval_smt_arith e1 v) (eval_smt_arith e2 v)
     end.
-
-(* Apply SmtValuation f to every entry in the symbolic state across all 3 maps *)
-Definition eval_sym_state (s: ProgramState SmtArithExpr) (f : SmtValuation) : ProgramState uint8 :=
-   let sym_eval := fun e => eval_smt_arith e f in
-   program_state_mapper sym_eval sym_eval sym_eval s.
